Cleanup the order on kernames and try an implemtation of the lookup environment with FMapAVLs instead of the canonical tries

safechecker/theories/PCUICEnvMap.v
@@ -1,15 +1,170 @@
 
 (* Distributed under the terms of the MIT license. *)
-From Coq Require Import ssreflect PArith.BinPos PArith.
-From MetaCoq.Template Require Import config utils uGraph Reflect String2pos CanonicalTries.
+From Coq Require Import ssreflect RelationClasses OrderedTypeAlt FMapAVL FMapFacts.
+From MetaCoq.Template Require Import config utils uGraph Reflect Kernames String2pos CanonicalTries.
 From MetaCoq.PCUIC Require Import PCUICAst PCUICAstUtils
      PCUICReflect PCUICTyping PCUICGlobalEnv PCUICTyping.
 From Equations Require Import Equations.
+Import String2pos.
 
 (* Implementation of environment lookup using efficient canonical tries by Appel & Leroy *)
 
 Implicit Types (cf:checker_flags).
 
+Module KernameMap := FMapAVL.Make KernameOT.OT.
+Module KernameMapFact := FMapFacts.WProperties KernameMap.
+
+Module EnvMap.
+  Definition t := KernameMap.t global_decl.
+
+  Definition empty : t := KernameMap.empty _.
+
+  Definition lookup (k : kername) (env : t) : option global_decl :=
+    KernameMap.find k env.
+
+  Definition add (k : kername) (g : global_decl) (env : t) : t :=
+    KernameMap.add k g env.
+
+  Definition of_global_env (g : global_env) : t :=
+    KernameMapFact.of_list g.
+
+  Lemma gso (e : t) kn kn' g : kn <> kn' ->
+    lookup kn (add kn' g e) = lookup kn e.
+  Proof.
+    intros ne.
+    unfold lookup, add.
+    rewrite KernameMapFact.F.add_neq_o //.
+    intros eq. apply KernameOT.compare_eq in eq. congruence.
+  Qed.
+
+  Lemma gss (e : t) kn kn' g : kn = kn' ->
+    lookup kn (add kn' g e) = Some g.
+  Proof.
+    intros eq.
+    unfold lookup, add.
+    rewrite KernameMapFact.F.add_eq_o //.
+    now apply KernameOT.compare_eq.
+  Qed.
+
+  Definition equal (g g' : t) := KernameMap.Equal g g'.
+    
+  Definition repr (g : global_env) (e : t) := 
+    equal e (of_global_env g).
+
+  Lemma repr_global_env (g : global_env) : repr g (of_global_env g).
+  Proof. red. reflexivity. Qed.
+
+  Lemma unfold_equal g g' : (forall i, lookup i g = lookup i g') -> equal g g'.
+  Proof.
+    intros heq.
+    intros i. apply heq.
+  Qed.
+
+  Lemma of_global_env_comm {cf:checker_flags} g d d' : 
+    fresh_global d.1 (d' :: g) -> fresh_global d'.1 g ->
+    equal (of_global_env (d :: d' :: g)) (of_global_env (d' :: d :: g)).
+  Proof.
+    intros hwf hwf'.
+    apply unfold_equal. intros i.
+    cbn -[lookup]. unfold KernameMapFact.uncurry.
+    destruct (eq_dec i d'.1).
+    - subst. rewrite gso. depelim hwf. apply H.
+      rewrite gss //. rewrite gss //.
+    - destruct (eq_dec i d.1); [subst i|].
+      + rewrite gss //. rewrite gso // gss //.
+      + rewrite !gso //.
+  Qed.
+
+  Lemma add_comm g d d' : 
+    d.1 <> d'.1 -> 
+    equal (add d.1 d.2 (add d'.1 d'.2 g)) (add d'.1 d'.2 (add d.1 d.2 g)).
+  Proof.
+    intros hwf.
+    cbn. apply unfold_equal.
+    intros i.
+    destruct (eq_dec i d'.1).
+    - subst. rewrite gso //. congruence.
+      rewrite gss // gss //.
+    - destruct (eq_dec i d.1); [subst i|].
+      + rewrite gss // gso // !gss //.
+      + rewrite !gso //.
+  Qed.
+
+  Inductive fresh_globals : global_env -> Prop :=
+    | fresh_globals_empty : fresh_globals []
+    | fresh_globals_cons kn d g : 
+      fresh_globals g -> fresh_global kn g ->
+      fresh_globals ((kn, d) :: g). 
+  Derive Signature for fresh_globals.
+
+  Lemma fold_left_cons d g acc :
+    fold_left (fun (genv : t) (decl : kername × global_decl) => add decl.1 decl.2 genv) (d :: g) acc = 
+    fold_left (fun (genv : t) (decl : kername × global_decl) => add decl.1 decl.2 genv) g (add d.1 d.2 acc).
+  Proof. reflexivity. Qed.
+  
+  Lemma of_global_env_cons {cf:checker_flags} d g : fresh_globals (d :: g) ->
+    of_global_env (d :: g) = add d.1 d.2 (of_global_env g).
+  Proof.
+    unfold of_global_env. simpl. unfold KernameMapFact.uncurry.
+    reflexivity.
+  Qed.
+  
+  Lemma wf_fresh_globals {cf} Σ : wf Σ -> fresh_globals Σ.
+  Proof. induction 1; constructor; auto. Qed.
+
+  Lemma repr_add {cf} {Σ : global_env} e k g : wf Σ ->
+    fresh_global k Σ ->
+    EnvMap.repr Σ e ->
+    EnvMap.repr ((k, g) :: Σ) (EnvMap.add k g e).
+  Proof.
+    intros wfΣ fresh repr.
+    red. rewrite /add. do 2 red in repr.
+    rewrite repr. rewrite of_global_env_cons //.
+    constructor => //. now apply wf_fresh_globals.
+  Qed.
+
+  Lemma lookup_add k v g : lookup k (add k v g) = Some v.
+  Proof. rewrite gss //. Qed.
+
+  Lemma lookup_add_other k k' v g : k <> k' -> lookup k (add k' v g) = lookup k g.
+  Proof. move=> eqk. rewrite gso //. Qed.
+
+  Lemma lookup_env_head d g : lookup_env (d :: g) d.1 = Some d.2.
+  Proof.
+    now rewrite /lookup_env eq_kername_refl.
+  Qed.
+
+  Lemma lookup_spec {cf : checker_flags} (g : global_env) (e : t) : wf g ->
+    repr g e ->
+    forall k, lookup k e = lookup_env g k.
+  Proof.
+    intros wf eq k. red in eq.
+    move: eq.
+    induction g in e, k, wf |- *; auto.
+    - simpl. intros eq.
+      unfold lookup.
+      rewrite -KernameMapFact.F.not_find_in_iff.
+      intros hin.
+      red in eq. rewrite eq in hin.
+      now eapply KernameMapFact.F.empty_in_iff in hin.
+    - cbn -[of_global_env].
+      change (eq_kername k a.1) with (eqb k a.1).
+      destruct (eqb_spec k a.1).
+      * subst. rewrite of_global_env_cons; [now apply wf_fresh_globals|].
+        intros he. unfold lookup. rewrite he.
+        now rewrite [KernameMap.find _ _]lookup_add.
+      * rewrite of_global_env_cons. now apply wf_fresh_globals.
+        intros he. unfold lookup. rewrite he.
+        rewrite [KernameMap.find _ _]lookup_add_other //.
+        apply IHg. now depelim wf.
+        reflexivity.
+  Qed.
+
+End EnvMap.
+
+Print Assumptions EnvMap.lookup_spec.
+
+(*
 Module EnvMap.
   Definition t := PTree.tree global_decl.
 
@@ -33,9 +188,16 @@ Module EnvMap.
     move/ascii_cons_pos_inj. intuition f_equal; auto.
   Qed.
 
+  Fixpoint pos_succ (p : positive) :=
+    match p with
+    | xH => xO xH
+    | xO p => xI p
+    | xI p => xO (pos_succ p)
+    end.
+
   Fixpoint pos_of_string_cont (s: string) (p : positive) : positive :=
     match s with
-    | EmptyString => Pos.succ p
+    | EmptyString => pos_succ p
     | String c s => ascii_cons_pos c (pos_of_string_cont s p)
     end.
 (*   
@@ -69,13 +231,13 @@ Module EnvMap.
 
  *)
 
-  Lemma pos_of_string_cont_spec s p : pos_of_string_cont s p = 
+  (* Lemma pos_of_string_cont_spec s p : pos_of_string_cont s p = 
     (Pos.shiftl (pos_of_string s) (N.of_nat (String.length s)) + p)%positive.
   Proof.
     induction s.
     - cbn. now destruct p; cbn.
     - cbn. rewrite IHs.
-  Admitted.
+  Admitted. *)
 
 
   Lemma pos_of_string_cont_inj s s' p : pos_of_string_cont s p = pos_of_string_cont s' p -> s = s'.
@@ -92,7 +254,7 @@ Module EnvMap.
   Fixpoint pos_of_nat_cont (n : nat) (cont : positive) : positive :=
     match n with
     | 0 => cont
-    | S x => Pos.succ (pos_of_nat_cont x cont)
+    | S x => pos_succ (pos_of_nat_cont x cont)
     end.
 
   Fixpoint pos_of_modpath_cont (m : modpath) (p : positive) : positive :=
@@ -136,12 +298,12 @@ Module EnvMap.
     cbn. f_equal. apply PTree.extensionality.
     intros i.
     unfold add.
-    destruct (Pos.eq_dec i (pos_of_kername d'.1)).
+    destruct (eq_dec i (pos_of_kername d'.1)).
     - subst. rewrite PTree.gss PTree.gso.
       intros eq. apply pos_of_kername_inj in eq. depelim hwf. cbn in H; congruence.
       now rewrite PTree.gss.
     - rewrite PTree.gso //.
-      destruct (Pos.eq_dec i (pos_of_kername d.1)); [subst i|].
+      destruct (eq_dec i (pos_of_kername d.1)); [subst i|].
       + rewrite !PTree.gss //.
       + rewrite !PTree.gso //.
   Qed.
@@ -151,11 +313,11 @@ Module EnvMap.
   Proof.
     intros hwf.
     cbn. unfold add. apply PTree.extensionality=> i.
-    destruct (Pos.eq_dec i (pos_of_kername d'.1)).
+    destruct (eq_dec i (pos_of_kername d'.1)).
     - subst. rewrite PTree.gss PTree.gso.
       intros eq. apply pos_of_kername_inj in eq. congruence.
       now rewrite PTree.gss.
-    - destruct (Pos.eq_dec i (pos_of_kername d.1)); [subst i|].
+    - destruct (eq_dec i (pos_of_kername d.1)); [subst i|].
       + rewrite !PTree.gss // PTree.gso // !PTree.gss //.
       + rewrite !PTree.gso //.
   Qed.
@@ -216,4 +378,4 @@ Module EnvMap.
       * apply IHg. now depelim wf.
   Qed.
 
-End EnvMap.
+End EnvMap. *)
